Prove trim_reduced and trim_evaluate

Bdd/Trim.lean
@@ -6,6 +6,18 @@ private def trim_pointer : Pointer m → Pointer (k + 1)
   | .terminal b => .terminal b
   | .node j => .node ⟨j.1 % (k + 1), Nat.mod_lt j.1 (Nat.zero_lt_succ k)⟩
 
+private lemma trim_pointer_injective {hp : ∀ j : Fin m, p = .node j → j.1 < l + 1} {hq : ∀ j : Fin m, q = .node j → j.1 < l + 1} :
+    trim_pointer (k := l) (m := m) p = trim_pointer q → p = q := by
+  intro h
+  cases p with
+  | terminal _ =>
+    cases q <;> simp_all [trim_pointer]
+  | node _ =>
+    cases q <;> simp_all [trim_pointer]
+    rw [Nat.mod_eq_of_lt hp] at h
+    rw [Nat.mod_eq_of_lt hq] at h
+    exact Fin.eq_of_val_eq h
+
 private def trim_node : Node n m → Node n (k + 1)
   | ⟨v, l, h⟩ => ⟨v, trim_pointer l, trim_pointer h⟩
 
@@ -22,6 +34,15 @@ def trim (B : Bdd n m) (h1 : k ≤ m) (h2 : ∀ j : Fin m, Pointer.Reachable B.h
 private def untrim_pointer (h : k ≤ m) : Pointer k → Pointer m
   | .terminal b => .terminal b
   | .node j => .node ⟨j.1, Fin.val_lt_of_le _ h⟩
+
+private lemma untrim_pointer_injective {h : k ≤ m} : Function.Injective (untrim_pointer h) := by
+  intro x y hxy
+  cases x with
+  | terminal _ =>
+    cases y <;> simp_all [untrim_pointer]
+  | node _ =>
+    cases y <;> simp_all [untrim_pointer]
+    exact Fin.eq_of_val_eq hxy
 
 private def untrim_node (h1 : k ≤ m) : Node n k → Node n m
   | ⟨v, l, h⟩ => ⟨v, untrim_pointer h1 l, untrim_pointer h1 h⟩
@@ -46,6 +67,23 @@ private lemma trim_induction {B : Bdd n m} {h1 : k ≤ m} {h2} {motive : ∀ k, 
     next b heq => exact base b heq
     next j heq => rw [heq] at h2; have := h2 j .refl; contradiction
   next l h1 h2 => exact step l h1 h2
+
+private lemma trim_root_terminal {B : Bdd n m} {h1 : k ≤ m} {h2} :
+    (trim B h1 h2).root = .terminal b → B.root = .terminal b := by
+  intro h
+  unfold trim at h
+  split at h
+  next h1 h2 =>
+    split at h
+    next => simp_all
+    next j hj =>
+      rw [hj] at h2
+      have := h2 j .refl
+      contradiction
+  next l h1 h2 =>
+    simp_all only [Nat.succ_eq_add_one]
+    simp [trim_pointer] at h
+    split at h <;> simp_all
 
 private lemma aux {n m} {B : Bdd n m} {l} {j} (h1 : l + 1 ≤ m) (h2 : j < l + 1) :
     ((Vector.map Trim.trim_node B.heap).extract 0 (l + 1))[j] =
@@ -253,12 +291,412 @@ lemma trim_ordered {B : Bdd n m} (o : B.Ordered) {h1 : k ≤ m} {h2} : (trim B h
 def otrim (O : OBdd n m) (h1 : k ≤ m) (h2 : ∀ j : Fin m, Pointer.Reachable O.1.heap O.1.root (.node j) → j < k) :
     OBdd n k := ⟨trim O.1 h1 h2, trim_ordered O.2⟩
 
-lemma otrim_reduced {O : OBdd n m} {h1 : k ≤ m} {h2} :
-    OBdd.Reduced O → OBdd.Reduced (otrim O h1 h2) := by
-  sorry
+private lemma otrim_noRedundancy {O : OBdd n m} {h1 : k ≤ m} {h2} (hr : O.1.NoRedundancy) : (otrim O h1 h2).1.NoRedundancy := by
+  rintro ⟨x, hx⟩ contra
+  cases contra with
+  | red hj =>
+    rename_i j
+    apply hr ⟨.node ⟨j.1, by omega⟩, (trim_reachable_and_edge hx).1⟩
+    constructor
+    simp only [otrim, Fin.getElem_fin] at hj
+    simp only [Fin.getElem_fin]
+    rw [← untrim_point_trim_heap_low (hj := (trim_reachable_and_edge hx).1)]
+    rw [← untrim_point_trim_heap_high (hj := (trim_reachable_and_edge hx).1)]
+    congr
+
+private lemma trim_root {B : Bdd n m} {h1 : l + 1 ≤ m} {h2} : (trim B h1 h2).root = trim_pointer B.root := by
+  simp only [trim]
+
+private def trim_root_node {h1 : k + 1 ≤ m} {h2} :
+    (trim B h1 h2).root = .node j → { j' // B.root = .node j' } := by
+  intro h
+  conv at h =>
+    lhs
+    rw [trim_root]
+  simp [trim_pointer] at h
+  split at h
+  next => contradiction
+  next j' hj' => use j'
+
+private def trim_root_node' {h1 : k + 1 ≤ m} {h2} :
+    (trim B h1 h2).root = .node j → B.root = .node ⟨j.1, by omega⟩ := by
+  intro h
+  conv at h =>
+    lhs
+    rw [trim_root]
+  simp [trim_pointer] at h
+  split at h
+  next => contradiction
+  next j' hj' =>
+    simp_all
+    rw [Fin.eq_mk_iff_val_eq] at h
+    simp_all only
+    apply Fin.eq_of_val_eq
+    simp only
+    rw [← h]
+    symm
+    simp only [Nat.mod_succ_eq_iff_lt, Nat.succ_eq_add_one]
+    apply h2
+    left
+
+private lemma otrim_low_aux {O : OBdd n m} {h : O.1.root = .node j} :
+    (∀ (j : Fin m), Pointer.Reachable O.1.heap O.1.root (Pointer.node j) → j.1 < k) →
+    (∀ (j : Fin m), Pointer.Reachable (O.low h).1.heap (O.low h).1.root (Pointer.node j) → j.1 < k) := by
+  intro h j' hj'
+  apply h
+  rw [OBdd.reachable_from_node_iff']
+  right
+  left
+  exact hj'
+
+private lemma otrim_high_aux {O : OBdd n m} {h : O.1.root = .node j} :
+    (∀ (j : Fin m), Pointer.Reachable O.1.heap O.1.root (Pointer.node j) → j.1 < k) →
+    (∀ (j : Fin m), Pointer.Reachable (O.high h).1.heap (O.high h).1.root (Pointer.node j) → j.1 < k) := by
+  intro h j' hj'
+  apply h
+  rw [OBdd.reachable_from_node_iff']
+  right
+  right
+  exact hj'
+
+private lemma trim_pointer_untrim_pointer {p : Pointer (l + 1)} (hp : ∀ j, p = .node j → j.1 < l + 1) {h1 : l + 1 ≤ m} :
+    Trim.trim_pointer (Trim.untrim_pointer h1 p) = p := by
+  cases h : p with
+  | terminal _ => simp [untrim_pointer, trim_pointer]
+  | node j =>
+    simp only [trim_pointer, untrim_pointer, Pointer.node.injEq]
+    have := hp j h
+    apply Fin.eq_of_val_eq
+    simp
+
+private lemma trim_reachable_reverse' {B : Bdd n m} {h1 : l + 1 ≤ m} {h2} :
+    Pointer.Reachable B.heap B.root p →
+    Pointer.Reachable (trim B h1 h2).heap (trim B h1 h2).root (trim_pointer p) ∧
+    (∀ q, Edge B.heap p q → Edge (trim B h1 h2).heap (trim_pointer p) (trim_pointer q)):= by
+  intro h
+  induction h with
+  | refl =>
+    constructor
+    · conv =>
+        congr
+        rfl
+        rfl
+        rw [← untrim_point_trim_root (h1 := h1) (h2 := h2)]
+      rw [trim_pointer_untrim_pointer]
+      left
+      intro j' hj'
+      have : B.root = .node ⟨j'.1, by omega⟩ := by
+        rw [trim_root] at hj'
+        simp [trim_pointer] at hj'
+        split at hj' <;> simp_all
+        rw [← hj']
+        apply Fin.eq_of_val_eq
+        simp only
+        rename_i j'' hj''
+        have := h2 j'' .refl
+        exact Eq.symm (Nat.mod_eq_of_lt this)
+      have := h2 ⟨j'.1, by omega⟩ (by rw [this]; left)
+      exact this
+    · intro q e
+      cases h : B.root with
+      | terminal _ => rw [h] at e; contradiction
+      | node j' =>
+        rcases B with ⟨heap, root⟩
+        cases e with
+        | low heq =>
+          left
+          simp_all only [Pointer.node.injEq, Fin.getElem_fin]
+          symm at h
+          subst h
+          rw [← heq]
+          simp only [trim, Nat.succ_eq_add_one, Vector.take_eq_extract, Vector.map_extract, Vector.getElem_cast]
+          have : j'.1 < l + 1 := by
+            apply h2
+            left
+          have : j'.1 % (l + 1) = j'.1 := Nat.mod_eq_of_lt this
+          simp_rw [this]
+          have := Vector.getElem_extract (as := (Vector.map (Trim.trim_node (k := l)) heap)) (n := m) (start := 0) (stop := l + 1) (i := j'.1) (by omega)
+          have : ((Vector.map (Trim.trim_node (k := l)) heap).extract 0 (l + 1))[↑j'].low = (Vector.map Trim.trim_node heap)[0 + ↑j'].low := by simp_all
+          simp at this
+          convert this
+        | high heq =>
+          right
+          simp_all only [Pointer.node.injEq, Fin.getElem_fin]
+          symm at h
+          subst h
+          rw [← heq]
+          simp only [trim, Nat.succ_eq_add_one, Vector.take_eq_extract, Vector.map_extract, Vector.getElem_cast]
+          have : j'.1 < l + 1 := by
+            apply h2
+            left
+          have : j'.1 % (l + 1) = j'.1 := Nat.mod_eq_of_lt this
+          simp_rw [this]
+          have := Vector.getElem_extract (as := (Vector.map (Trim.trim_node (k := l)) heap)) (n := m) (start := 0) (stop := l + 1) (i := j'.1) (by omega)
+          have : ((Vector.map (Trim.trim_node (k := l)) heap).extract 0 (l + 1))[↑j'].high = (Vector.map Trim.trim_node heap)[0 + ↑j'].high := by simp_all
+          simp at this
+          convert this
+  | tail r e ih =>
+    constructor
+    · right
+      exact ih.1
+      exact ih.2 _ e
+    · intro q hq
+      cases hq with
+      | low hq =>
+        nth_rw 1 [trim_pointer]
+        left
+        rename_i j
+        have hj : Pointer.Reachable B.heap B.root (Pointer.node j) := .tail r e
+        have : j.1 < l + 1 := h2 _ hj
+        have := untrim_point_trim_heap_low (j := ⟨j.1, by omega⟩) (h2 := h2) (hj := hj) (h1 := h1)
+        simp at this
+        simp at hq
+        conv at hq =>
+          lhs
+          rw [← this]
+        rw [← hq]
+        simp [trim_pointer_untrim_pointer]
+        congr
+        simpa
+      | high _ =>
+        nth_rw 1 [trim_pointer]
+        right
+        rename_i j hq
+        have hj : Pointer.Reachable B.heap B.root (Pointer.node j) := .tail r e
+        have : j.1 < l + 1 := h2 _ hj
+        have := untrim_point_trim_heap_high (j := ⟨j.1, by omega⟩) (h2 := h2) (hj := hj) (h1 := h1)
+        simp at this
+        simp at hq
+        conv at hq =>
+          lhs
+          rw [← this]
+        rw [← hq]
+        simp [trim_pointer_untrim_pointer]
+        congr
+        simpa
+
+private lemma trim_reachable_reverse {B : Bdd n m} {h1 : l + 1 ≤ m} {j : Fin (l + 1)} {h2} :
+    Pointer.Reachable B.heap B.root (Pointer.node ⟨j, by omega⟩) →
+    Pointer.Reachable (trim B h1 h2).heap (trim B h1 h2).root (Pointer.node j) := by
+  intro h
+  have := (trim_reachable_reverse' (B := B) (h1 := h1) (h2 := h2) (p := (Pointer.node ⟨j, by omega⟩)) h).1
+  convert this
+  simp only [trim_pointer, Pointer.node.injEq]
+  apply Fin.eq_of_val_eq
+  have := h2 ⟨j.1, by omega⟩ h
+  exact Eq.symm (Nat.mod_eq_of_lt this)
+
+@[simp]
+private lemma trim_low {B : Bdd n m} {h1 : l + 1 ≤ m} {h2} {j : Fin (l + 1)} {hj : Pointer.Reachable B.heap B.root (Pointer.node ⟨j.1, by omega⟩)}:
+    (trim B h1 h2).heap[j.1].low = trim_pointer B.heap[j.1].low := by
+  conv =>
+    rhs
+    congr
+    rw [← untrim_point_trim_heap_low (h1 := h1) (B := B) (h2 := h2) (hj := hj)]
+  rw [trim_pointer_untrim_pointer]
+  intro j' hj'
+  apply h2 ⟨j', by omega⟩
+  have : Pointer.Reachable (trim B h1 h2).heap (trim B h1 h2).root (.node j') := by
+    right
+    exact trim_reachable_reverse hj
+    left
+    exact hj'
+  have := (trim_reachable_and_edge this).1
+  simp only [untrim_pointer] at this
+  exact this
+
+@[simp]
+private lemma trim_high {B : Bdd n m} {h1 : l + 1 ≤ m} {h2} {j : Fin (l + 1)} {hj : Pointer.Reachable B.heap B.root (Pointer.node ⟨j.1, by omega⟩)}:
+    (trim B h1 h2).heap[j.1].high = trim_pointer B.heap[j.1].high := by
+  conv =>
+    rhs
+    congr
+    rw [← untrim_point_trim_heap_high (h1 := h1) (B := B) (h2 := h2) (hj := hj)]
+  rw [trim_pointer_untrim_pointer]
+  intro j' hj'
+  apply h2 ⟨j', by omega⟩
+  have : Pointer.Reachable (trim B h1 h2).heap (trim B h1 h2).root (.node j') := by
+    right
+    exact trim_reachable_reverse hj
+    right
+    exact hj'
+  have := (trim_reachable_and_edge this).1
+  simp only [untrim_pointer] at this
+  exact this
+
+private lemma otrim_low {O : OBdd n m} {h1 : l + 1 ≤ m} {h2} {h : (otrim O h1 h2).1.root = .node j} :
+    (otrim O h1 h2).low h = (otrim (O.low (trim_root_node' (h1 := h1) (h2 := h2) (j := j) (by simp_all [otrim]))) h1 (otrim_low_aux h2)) := by
+  simp only [OBdd.low, Bdd.low, otrim, Fin.getElem_fin]
+  congr
+  simp only
+  apply trim_low
+  simp [otrim] at h
+  rw [← untrim_point_trim_root (h1 := h1) (h2 := h2)]
+  rw [h]
+  left
+
+private lemma otrim_high {O : OBdd n m} {h1 : k + 1 ≤ m} {h2} {h : (otrim O h1 h2).1.root = .node j} :
+    (otrim O h1 h2).high h = (otrim (O.high (trim_root_node' (h1 := h1) (h2 := h2) (j := j) (by simp_all [otrim]))) h1 (otrim_high_aux h2)) := by
+  simp only [OBdd.high, Bdd.high, otrim, Fin.getElem_fin]
+  congr
+  simp only
+  apply trim_high
+  simp [otrim] at h
+  rw [← untrim_point_trim_root (h1 := h1) (h2 := h2)]
+  rw [h]
+  left
+
+private lemma trim_var {B : Bdd n m} {h1 : l + 1 ≤ m} {h2} {j : Fin (l + 1)} {hj : Pointer.Reachable B.heap B.root (Pointer.node ⟨j.1, by omega⟩)} :
+    (trim B h1 h2).heap[j.1].var = B.heap[j.1].var := by
+  apply trim_induction (motive := fun k T ↦ ∀ (hk : k = l + 1), T.heap[j.1].var = B.heap[j].var)
+  · simp
+  · intro l' h1' h2' hk
+    simp only [Nat.add_right_cancel_iff] at hk
+    symm at hk
+    subst hk
+    simp only [Vector.take_eq_extract, Vector.map_extract, Vector.getElem_cast, Fin.getElem_fin]
+    have : j.1 < l + 1 := by
+      have := h2' ⟨j.1, by omega⟩ hj
+      simp only at this
+      exact this
+    have := Vector.getElem_extract (as := (Vector.map (Trim.trim_node (k := l)) B.heap)) (n := m) (start := 0) (stop := l + 1) (i := j.1) (by omega)
+    simp at this
+    rw [this]
+    simp [trim_node]
+    congr
+  · simp
+
+private lemma otrim_toTree' {O : OBdd n m} {h1 : l + 1 ≤ m} {h2} :
+    OBdd.toTree (otrim O h1 h2) = OBdd.toTree O := by
+  cases heq : (otrim O h1 h2).1.root with
+  | terminal b =>
+    have : O.1.root = .terminal b := by
+      simp only [otrim] at heq
+      simp only [trim] at heq
+      simp [trim_pointer] at heq
+      split at heq
+      next => simp_all
+      next => simp at heq
+    simp only [OBdd.toTree_terminal' heq]
+    simp only [OBdd.toTree_terminal' this]
+  | node j =>
+    rw [OBdd.toTree_node heq]
+    conv =>
+      lhs
+      rw [otrim_low]
+      rw [otrim_high]
+    rw [OBdd.toTree_node (trim_root_node' heq (h1 := h1) (h2 := h2))]
+    congr 1
+    · have hj : Pointer.Reachable O.1.heap O.1.root (Pointer.node ⟨j.1, by omega⟩) := by
+        simp only [otrim] at heq
+        rw [trim_root] at heq
+        have := trim_pointer_untrim_pointer (l := l) (h1 := h1) (p := (Pointer.node ⟨j.1, by omega⟩)) ?_
+        · rw [← this] at heq
+          have := trim_pointer_injective
+            (p := O.1.root)
+            (q := (Trim.untrim_pointer h1 (Pointer.node ⟨↑j, by omega⟩)))
+            (hp := by intro j' hj'; apply h2; rw [hj']; left)
+            (hq := fun j' hj' ↦ by
+              simp only [untrim_pointer, Pointer.node.injEq] at hj'
+              rw [Fin.eq_mk_iff_val_eq] at hj'
+              simp_all
+              omega
+            )
+            (l := l) heq
+          rw [this]
+          left
+        · intro j' hj'
+          omega
+      exact trim_var (hj := hj) (h2 := h2) (h1 := h1)
+    · exact otrim_toTree'
+    · exact otrim_toTree'
+termination_by O
+
+private lemma otrim_toTree {h1 : l + 1 ≤ m} (hx : Pointer.Reachable (otrim O h1 h2).1.heap (otrim O h1 h2).1.root x) :
+    OBdd.toTree ⟨⟨(otrim O h1 h2).1.heap, x⟩, Bdd.ordered_of_reachable hx⟩ =
+    OBdd.toTree ⟨⟨O.1.heap, Trim.untrim_pointer h1 x⟩, Bdd.ordered_of_reachable (trim_reachable_and_edge hx).1⟩ := by
+  induction hx with
+  | refl =>
+    have : OBdd.toTree ⟨{ heap := (otrim O h1 h2).1.heap, root := (otrim O h1 h2).1.root }, trim_ordered O.2 (h1 := h1) (h2 := h2)⟩ = (otrim O h1 h2).toTree := rfl
+    rw [this]
+    rw [otrim_toTree']
+    simp only [otrim]
+    simp_rw [untrim_point_trim_root]
+    rfl
+  | tail r e ih =>
+    rename_i b c
+    cases b with
+    | terminal b => contradiction
+    | node j =>
+      simp [untrim_pointer] at ih
+      rw [OBdd.toTree_node rfl] at ih
+      conv at ih =>
+        rhs
+        rw [OBdd.toTree_node rfl]
+      injection ih with hv hl hh
+      cases e with
+      | low heq =>
+        convert hl
+        · simp only [OBdd.low, Bdd.low, Fin.getElem_fin]
+          simp only [Fin.getElem_fin] at heq
+          simp_rw [heq]
+        · simp only [OBdd.low, Bdd.low, Fin.getElem_fin]
+          simp only [Fin.getElem_fin] at heq
+          simp_rw [← heq]
+          simp only [otrim]
+          congr
+          rw [untrim_point_trim_heap_low]
+          exact (trim_reachable_and_edge r (h2 := h2) (h1 := h1)).1
+      | high heq =>
+        convert hh
+        · simp only [OBdd.high, Bdd.high, Fin.getElem_fin]
+          simp only [Fin.getElem_fin] at heq
+          simp_rw [heq]
+        · simp only [OBdd.high, Bdd.high, Fin.getElem_fin]
+          simp only [Fin.getElem_fin] at heq
+          simp_rw [← heq]
+          simp only [otrim]
+          congr
+          rw [untrim_point_trim_heap_high]
+          exact (trim_reachable_and_edge r (h2 := h2) (h1 := h1)).1
+
+private lemma otrim_similarRp {h1 : l + 1 ≤ m}:
+    (otrim O h1 h2).SimilarRP ⟨x, hx⟩ ⟨y, hy⟩ →
+    O.SimilarRP ⟨Trim.untrim_pointer h1 x, (trim_reachable_and_edge hx).1⟩ ⟨Trim.untrim_pointer h1 y, (trim_reachable_and_edge hy).1⟩ := by
+  simp only [OBdd.SimilarRP, OBdd.Similar, OBdd.HSimilar]
+  intro h
+  rw [otrim_toTree hx] at h
+  rw [otrim_toTree hy] at h
+  exact h
+
+private lemma otrim_reduced_helper {O : OBdd n m} {h1 : l + 1 ≤ m} {h2} (hr : Subrelation (OBdd.SimilarRP O) (InvImage Eq Subtype.val)) :
+    Subrelation (OBdd.SimilarRP (otrim O h1 h2)) (InvImage Eq Subtype.val) := by
+  intro ⟨x, hx⟩ ⟨y, hy⟩ hxy
+  simp only [InvImage]
+  have : untrim_pointer h1 x = untrim_pointer h1 y := by
+    refine @hr
+      ⟨(untrim_pointer h1 x), (trim_reachable_and_edge (h2 := h2) hx).1⟩
+      ⟨(untrim_pointer h1 y), (trim_reachable_and_edge (h2 := h2) hy).1⟩
+      ?_
+    apply (otrim_similarRp (h1 := h1) (h2 := h2) hxy) <;> simp_all
+  exact untrim_pointer_injective this
+
+lemma otrim_reduced {O : OBdd n m} {h1 : k ≤ m} {h2} (hr : OBdd.Reduced O) :
+    OBdd.Reduced (otrim O h1 h2) :=
+  match k with
+  | .zero => OBdd.reduced_of_terminal (Bdd.terminal_of_zero_heap (B := (otrim O h1 h2).1) (m := 0) rfl)
+  | .succ _ => ⟨otrim_noRedundancy hr.1, otrim_reduced_helper hr.2⟩
 
 lemma otrim_evaluate {O : OBdd n m} {h1 : k ≤ m} {h2} :
     OBdd.evaluate (otrim O h1 h2) = O.evaluate := by
-  sorry
+  cases k with
+  | zero =>
+    have := (Bdd.terminal_of_zero_heap (B := (otrim O h1 h2).1) (m := 0) rfl)
+    rcases this with ⟨b, hb⟩
+    rw [OBdd.evaluate_terminal' hb]
+    simp only [otrim] at hb
+    have := trim_root_terminal hb
+    rw [OBdd.evaluate_terminal' this]
+  | succ _ => simp only [OBdd.evaluate, Function.comp_apply, otrim_toTree']
 
 end Trim
